theories/Substitution/Introductions/Quote.v
@@ -1,0 +1,169 @@
+From LogRel.AutoSubst Require Import core unscoped Ast Extra.
+From LogRel Require Import Utils BasicAst Notations Context Closed NormalForms NormalEq Weakening UntypedReduction
+  DeclarativeTyping GenericTyping LogicalRelation Validity.
+From LogRel.LogicalRelation Require Import Escape Reflexivity Neutral Weakening Irrelevance Application Reduction Transitivity NormalRed.
+From LogRel.Substitution Require Import Irrelevance Properties SingleSubst.
+From LogRel.Substitution.Introductions Require Import Universe Nat SimpleArr.
+
+Set Universe Polymorphism.
+Set Printing Primitive Projection Parameters.
+
+Section QuoteValid.
+
+Context `{GenericTypingProperties}.
+Context {SN : SNTypingProperties ta _ _ _ _ _}.
+
+Lemma nf_eval : forall {l Γ A t} {vA : [Γ ||-<l> A]}, [vA | Γ ||- t : A] ->
+  ∑ r, [t ⇶* r] × dnf r × [Γ |- t ≅ r : A].
+Proof.
+intros l Γ A t vT vt.
+destruct SN as [sn].
+apply reflLRTmEq, escapeEqTerm, sn in vt.
+destruct vt as (t₀&u₀&[]&[]&?&?&?).
+exists t₀; try now prod_splitter.
+Qed.
+
+  Lemma QuoteRedEq : forall Γ l t t' (rΓ : [|- Γ]) (rNat := natRed rΓ),
+    [Γ |- t : arr tNat tNat] ->
+    [Γ |- t' : arr tNat tNat] ->
+    [Γ ||-<l> t ≅ t' : arr tNat tNat | SimpleArr.ArrRedTy rNat rNat ] ->
+    [Γ ||-<l> tQuote t ≅ tQuote t' : tNat | rNat ].
+  Proof.
+  intros * rt rt' re.
+  assert [Γ |- t ≅ t' : arr tNat tNat] by now eapply escapeEqTerm.
+  apply escapeEqTerm, snty_nf in re.
+  destruct re as (l₀&r₀&[]&[]&?&?&?).
+  remember (is_closedn 0 l₀) as b eqn:Hc; symmetry in Hc.
+  assert (Hc' : is_closedn 0 r₀ = b).
+  { erewrite eqnf_is_closedn; [tea|now apply Symmetric_eqnf]. }
+  destruct b.
+  - exists tZero tZero.
+    + constructor; [gen_typing|].
+      transitivity (tQuote l₀).
+      * apply redtm_quote; tea.
+      * apply redtm_eval; tea.
+        now eapply urefl.
+    + constructor; [gen_typing|].
+      transitivity (tQuote r₀).
+      * apply redtm_quote; tea.
+      * apply redtm_eval; tea.
+        now eapply urefl.
+    + gen_typing.
+    + constructor.
+  - assert [Γ |-[ ta ] tQuote l₀ ~ tQuote r₀ : tNat].
+    { apply convneu_quote; tea.
+      + etransitivity; [now symmetry|].
+        etransitivity; tea.
+      + unfold closed0; destruct is_closedn; cbn; congruence.
+      + unfold closed0; destruct is_closedn; cbn; congruence. }
+    exists (tQuote l₀) (tQuote r₀).
+    + constructor; [now eapply ty_quote, urefl|].
+      apply redtm_quote; tea.
+    + constructor; [now eapply ty_quote, urefl|].
+      apply redtm_quote; tea.
+    + apply convtm_convneu; tea.
+    + constructor; constructor; tea.
+  Qed.
+
+  Context {Γ l t} (vΓ : [||-v Γ])
+    (vNat := natValid (l := l) vΓ)
+    (vArr := simpleArrValid vΓ vNat vNat)
+    (vt : [ Γ ||-v< l > t : arr tNat tNat | vΓ | vArr ])
+  .
+
+  Lemma QuoteValid : [ Γ ||-v< l > tQuote t : tNat | vΓ | vNat ].
+  Proof.
+    econstructor.
+    - intros Δ σ tΔ vσ; cbn in *.
+      destruct vt as [vt0 vte].
+      specialize (vt0 _ _ _ vσ).
+      assert (Hv : [Δ |- t[σ] : arr tNat tNat]).
+      { now eapply escapeTerm. }
+      destruct (nf_eval vt0) as [r [Hdnf [Hr Hconv]]].
+      assert ([Δ |- tQuote t[σ] ⤳* tQuote r : tNat]).
+      { apply redtm_quote; tea. }
+      assert [Δ |- r ≅ r : arr tNat tNat].
+      { etransitivity; [symmetry|]; tea. }
+      assert [Δ |- tQuote r : tNat ].
+      { now apply ty_quote. }
+      pose (c := is_closedn 0 r); assert (is_closedn 0 r = c) as Hc by reflexivity; destruct c.
+      + exists tZero; [|gen_typing|constructor].
+        constructor.
+        { now apply ty_zero. }
+        { transitivity (tQuote r); [tea|].
+          now apply redtm_eval. }
+      + assert (~ closed0 r).
+        { unfold closed0; intros; destruct is_closedn; congruence. }
+        exists (tQuote r).
+        * split; [|tea].
+          now apply ty_quote.
+        * apply convtm_convneu, convneu_quote; tea.
+        * apply NatRedTm.neR; constructor; tea.
+          now apply convneu_quote.
+  - intros Δ σ σ' tΔ vσ vσ' vσσ'; cbn.
+    destruct vt as [vt0 vte].
+    assert [Δ |- t[σ] : arr tNat tNat].
+    { unshelve eapply escapeTerm, vt0; tea. }
+    assert [Δ |- t[σ'] : arr tNat tNat].
+    { unshelve eapply escapeTerm, vt0; tea. }
+    unshelve eapply QuoteRedEq, LRTmEqIrrelevant', vte; cbn; tea.
+    reflexivity.
+  Qed.
+
+Lemma evalValid : dnf t -> closed0 t ->
+  [Γ ||-v<l> tQuote t ≅ tZero : tNat | vΓ | vNat].
+Proof.
+destruct SN as [sn].
+econstructor.
+intros Δ σ tΔ vσ.
+destruct vt as [vt0 vte]; cbn.
+assert (vtt0 := vt0 Δ σ tΔ vσ).
+unshelve eassert (vte0 := vte Δ σ σ tΔ vσ vσ _).
+{ apply reflSubst. }
+apply escapeEqTerm, sn in vte0 as (t₀&u₀&[]&[]&?&?&?); cbn in *.
+assert [Δ |-[ ta ] t[σ] : tProd tNat tNat].
+{ eapply escapeTerm, vtt0. }
+exists tZero tZero; cbn in *.
+- constructor; [gen_typing|].
+  transitivity (tQuote t₀).
+  + apply redtm_quote; tea.
+  + apply redtm_eval; tea.
+    * now eapply urefl.
+    * eapply dredalg_closed0; [tea|].
+      now eapply closed0_subst.
+- constructor; [gen_typing|].
+  apply redtm_refl; gen_typing.
+- gen_typing.
+- constructor.
+Qed.
+
+End QuoteValid.
+
+Section QuoteCongValid.
+
+Context `{GenericTypingProperties}.
+Context {SN : SNTypingProperties ta _ _ _ _ _}.
+
+Context {Γ l t t'}
+  (vΓ : [||-v Γ])
+  (vNat := natValid (l := l) vΓ)
+  (vArr := simpleArrValid vΓ vNat vNat)
+  (vt : [Γ ||-v<l> t : arr tNat tNat | vΓ | vArr])
+  (vt' : [Γ ||-v<l> t' : arr tNat tNat | vΓ | vArr])
+.
+
+Lemma QuoteCongValid :
+  [Γ ||-v<l> t ≅ t' : arr tNat tNat | vΓ | vArr] ->
+  [Γ ||-v<l> tQuote t ≅ tQuote t' : tNat | vΓ | vNat].
+Proof.
+intros [vte]; constructor.
+intros Δ σ tΔ vσ; cbn.
+assert [Δ |- t[σ] : arr tNat tNat].
+{ unshelve eapply escapeTerm, vt; tea. }
+assert [Δ |- t'[σ] : arr tNat tNat].
+{ unshelve eapply escapeTerm, vt'; tea. }
+unshelve eapply QuoteRedEq, LRTmEqIrrelevant', vte; cbn; tea.
+reflexivity.
+Qed.
+
+End QuoteCongValid.
